% hh
b.\ \  $A$表象到$B$表象的变换矩阵$S$

通过矩阵$A$，求解$A|a \rangle=a|a \rangle$，得到$A$的本征态为
$$
\begin{array}{l}
|1\rangle_{a}=\frac{1}{\sqrt{2}}\left(\begin{array}{l}
1 \\
0
\end{array}\right), \quad|-1\rangle_{a}=\frac{1}{\sqrt{2}}\left(\begin{array}{l}
0 \\
1
\end{array}\right)
\end{array}
$$
从表象$A$到表象$B$的幺正变换矩阵元为$_a\langle a|b\rangle _b$，计算如下
$$
\begin{array}{l}
	\left. S_{11}=_a\langle 1|1\rangle _b=(1,0)\frac{1}{\sqrt{2}}\left( \begin{array}{c}
	1\\
	e^{-i\delta}\\
\end{array} \right) =\frac{1}{\sqrt{2}} \right.\\
	S_{21}=_a\langle -1|1\rangle _b=(0,1)\frac{1}{\sqrt{2}}\left( \begin{array}{c}
	1\\
	e^{-i\delta}\\
\end{array} \right) =\frac{1}{\sqrt{2}}e^{-i\delta}\\
	S_{12}=_a\langle 1|-1\rangle _b=(1,0)\frac{1}{\sqrt{2}}\left( \begin{array}{c}
	1\\
	-e^{-i\delta}\\
\end{array} \right) =\frac{1}{\sqrt{2}}\\
	S_{22}=_a\langle -1|-1\rangle _b=(0,1)\frac{1}{\sqrt{2}}\left( \begin{array}{c}
	1\\
	-e^{-i\delta}\\
\end{array} \right) =\frac{1}{\sqrt{2}}\left( -e^{-i\delta} \right)\\
\end{array}
$$
故
$$
S=\frac{1}{\sqrt{2}}\left(\begin{array}{cc}
1 & 1 \\
\mathrm{e}^{-\mathrm{i} \delta} & -\mathrm{e}^{-\mathrm{i} \delta}
\end{array}\right)
$$
$$
\left\{ \begin{array}{l}
	\hat{A}^2=\hat{B}^2=1\\
	\hat{A}\hat{B}+\hat{B}\hat{A}=0\\
\end{array} \right. 
$$
$\bm{}$
